X\sim\mathrm{}\left(\right)\\
x\in\mathbb{N}\\
\in\mathbb{N}\\
F_{X}\left(x\right)=\\
f_{X}\left(x\right)=\\
F^{-1}_{X}\left(u\right)=\\
E[X^k]=\mu'_{k}=\sum_{x=0}^{1}x^{k}f_{X}\left(x\right)\\
\mathrm{Mean}(X)=\mu'_{1}\\
\mathrm{Variance}(X)=(\mu'_{2}-\mu'^{2}_{1})\\
\mathrm{Skewness}(X)=\frac{\mu'_{3}-3\mu'_{2}\mu'_{1}+2\mu'^{3}_{1}}{(\mu'_{2}-\mu'^{2}_{1})^{1.5}}\\
\mathrm{Kurtosis}(X)=\frac{\mu'_{4}-4\mu'_{1}\mu'_{3}+6\mu'^{2}_{1}\mu'_{2}-3\mu'^{4}_{1}}{(\mu'_{2}-\mu'^{2}_{1})^{2}}\\
\mathrm{Median}(X)=\\
\mathrm{Mode}(X)=\\

L:\text{Location parameter}\\
S:\text{Scale parameter}\\
z\left(x\right)=\left(x-L\right)/S\\
z\left(x\right)=\left(x-min\right)/\left(max-min\right)\\
u:\text{Uniform[0,1] random varible}\\
\Phi\left(x\right):\text{Cumulative function from standard normal distribution}\\
\phi\left(x\right):\text{Density function from standard normal distribution}\\
\mathrm{erf}(x):\text{Error function}\\
\Phi^{-1}\left(x\right):\text{Inverse of cumulative function from standard normal distribution}\\
\mathrm{erf}^{-1}(x):\text{Inverse of error function}\\
I_{\alpha}\left(x\right):\text{Modified Bessel function of the first kind of order }\alpha\in\mathbb{N}\\
P\left(a,x\right)=\frac{\gamma(a,x)}{\Gamma(a)}:\text{Regularized lower incomplete gamma function}\\
P^{-1}\left(a,u\right):\text{Inverse of regularized lower incomplete Gamma function}\\
\gamma\left(a,x\right):\text{Lower incomplete Gamma function}\\
\Gamma\left(x\right):\text{Gamma function}\\
I\left(x,a,b\right):\text{Regularized incomplete Beta function}\\
I^{-1}\left(x,a,b\right):\text{Inverse of regularized incomplete Beta function}\\
Beta\left(x,y\right):\text{Beta function}\\
\gamma:\text{Euler–Mascheroni constant}=0.5772156649\\
\zeta(3):\text{Apéry's constant}=1.2020569031\\
\psi_{0}\left(x\right):\text{Digamma function}\\
\psi_{n}\left(x\right):\text{Polygamma function of order }n\in\mathbb{N}\\
\lfloor{x}\rfloor: \text{Floor function}\\
\lceil{x}\rceil: \text{Ceiling Function}\\
S(a,b):\text{Stirling numbers of the second kind}=\frac1{b!}\sum_{j=0}^b(-1)^{b-j}\binom {b}{j} j^a\\